% Automatically generated
\csname tex4ht\endcsname
\HCode{\Hnewline \Hnewline <!-- tex4ht_begin sing_tex4ht_displaymath displaymath 1 -->\Hnewline}

$$disp--laymath
f(x) = {1 \over \sigma \sqrt{2\pi}}e@sup{-{1 \over 2}\left({x-\mu \over \sigma}\right)^2}
$$
\HCode{\Hnewline <!-- tex4ht_end sing_tex4ht_displaymath displaymath 1 -->\Hnewline \Hnewline}
\HCode{\Hnewline \Hnewline <!-- tex4ht_begin sing_tex4ht_displaymath displaymath 2 -->\Hnewline}

$$disp--laymath
f(x) = {1 \over \sigma \sqrt{2\pi}}e@sup{-{1 \over 2}\left({x-\mu \over \sigma}\right)^2}
$$
\HCode{\Hnewline <!-- tex4ht_end sing_tex4ht_displaymath displaymath 2 -->\Hnewline \Hnewline}
\HCode{\Hnewline \Hnewline <!-- tex4ht_begin sing_tex4ht_displaymath displaymath 3 -->\Hnewline}

$$disp--laymath
f(x) = {1 \over \sigma \sqrt{2\pi}}e@sup{-{1 \over 2}\left({x-\mu \over \sigma}\right)^2}
$$
\HCode{\Hnewline <!-- tex4ht_end sing_tex4ht_displaymath displaymath 3 -->\Hnewline \Hnewline}
\HCode{\Hnewline \Hnewline <!-- tex4ht_begin sing_tex4ht_displaymath displaymath 4 -->\Hnewline}

$$disp--laymath
f(x) = {1 \over \sigma \sqrt{2\pi}}e@sup{-{1 \over 2}\left({x-\mu \over \sigma}\right)^2}
$$
\HCode{\Hnewline <!-- tex4ht_end sing_tex4ht_displaymath displaymath 4 -->\Hnewline \Hnewline}

\bye
